@prefix owl: <http://www.w3.org/2002/07/owl#> .
@prefix rdf: <http://www.w3.org/1999/02/22-rdf-syntax-ns#> .
@prefix sto: <https://w3id.org/i40/sto#> .
@prefix rdfs: <http://www.w3.org/2000/01/rdf-schema#> .
@prefix sh: <http://www.w3.org/ns/shacl#> .
@prefix xsd: <http://www.w3.org/2001/XMLSchema#> .
@prefix dcterms: <http://purl.org/dc/terms/> .
@prefix skos: <http://www.w3.org/2004/02/skos/core#> .
@prefix lingg: <http://purl.org/linguistics/gold/> .


sto:SmallClassShape
    a sh:NodeShape ; 
    rdfs:label "Small Class Shape" ;
    rdfs:comment "This shape checks that all classes have at least a label (@en or xsd:string) and a comment in english."@en ;
    sh:targetClass owl:Class ;


    sh:property [
      rdfs:comment "This is an unnecessary repetition of the shape's target clause and will always be true."@en ;
      sh:path rdf:type ;
      sh:minCount 1 ;
    ] ;
    
    sh:or 
    (
      [ sh:path rdfs:label ;
        sh:datatype rdf:langString ;]
      [ sh:path rdfs:label ;
        sh:datatype xsd:string ;]
    ) ;

    sh:property [
      sh:path rdfs:comment ;
      sh:datatype rdf:langString ;
      sh:minCount 1 ;
    ] ;
    
    .

sto:SmallPropertyShape
    a sh:NodeShape ; 
    rdfs:label "Small Property Shape" ;
    rdfs:comment "This shape checks that all properties have at least a label (@en or xsd:string), a comment in english, and some other stuff."@en ;
    sh:targetClass rdf:Property ;

    sh:property [
      rdfs:comment "This is an unnecessary repetition of the shape's target clause and will always be true."@en ;
      sh:path rdf:type ;
      sh:minCount 1 ;
    ] ;
    
    sh:or 
    (
      [ sh:path rdfs:label ;
        sh:datatype rdf:langString ;]
      [ sh:path rdfs:label ;
        sh:datatype xsd:string ;]
    ) ;

    sh:property [
      sh:path rdfs:comment ;
      sh:datatype rdf:langString ;
      sh:minCount 1 ;
    ] ;

    sh:property [
      sh:path rdfs:domain ;
      sh:maxCount 1 ;
    ] ;

    sh:property [
      sh:path rdfs:range ;
      sh:maxCount 1 ;
    ] ;
    
    .

sto:SmallInstanceShape
    a sh:NodeShape ; 
    rdfs:label "Small Instance Shape" ;
    rdfs:comment "This shape checks that all instances have at least a label (@en or xsd:string)."@en ;
    sh:targetClass rdf:Property ;

    sh:property [
      rdfs:comment "This is an unnecessary repetition of the shape's target clause and will always be true."@en ;
      sh:path rdf:type ;
      sh:minCount 1 ;
    ] ;
    
    sh:or 
    (
      [ sh:path rdfs:label ;
        sh:datatype rdf:langString ;]
      [ sh:path rdfs:label ;
        sh:datatype xsd:string ;]
    ) ;

    sh:property [
      sh:path rdfs:comment ;
      sh:datatype rdf:langString ;
      sh:minCount 1 ;
    ] ;
    
    .


# Basic entailment axioms:
owl:DatatypeProperty rdfs:subClassOf rdf:Property .
owl:AnnotationProperty rdfs:subClassOf rdf:Property .
owl:ObjectProperty rdfs:subClassOf rdf:Property .

owl:Class rdfs:subClassOf rdf:Resource .
owl:NamedIndividual rdfs:subClassOf rdf:Resource .
owl:Property rdfs:subClassOf rdf:Resource .